Cleaning and reordering files

cogent/examples/repeat/RepeatMono.thy
@@ -1,10 +1,19 @@
 theory RepeatMono
-  imports RepeatValue
+  imports Cogent.Mono RepeatValue
 begin
 
-definition vrepeatp
+section "Repeat loop definition"
+
+text "Wrapper with extra checks:
+  Summary:
+    Checks the arguments are of the correct form and then passes these to
+    @{term vrepeat_bod} with minor processing.
+  Checks:
+    * The functions f and g are of the form."
+
+definition prepeat
   where
-"vrepeatp \<xi>' x y =
+"prepeat \<xi>' x y =
   (\<exists>n f g acc obsv ret.
     x = VRecord [VPrim (LU64 n), f, g, acc, obsv] \<and>
     y = ret \<and>
@@ -12,13 +21,7 @@ definition vrepeatp
     is_vvalfun g \<and>
     vrepeat_bod \<xi>' (unat n) (vvalfun_to_expr f) (vvalfun_to_expr g) acc obsv ret)"
 
-definition \<xi>p0 :: "'b \<Rightarrow> ('b, 'c) vval \<Rightarrow> ('b, 'c) vval \<Rightarrow> bool"
-  where
-"\<xi>p0 f x y = False"
-
-definition \<xi>p1 :: "funtyp \<Rightarrow> (funtyp, 'c) vval \<Rightarrow> (funtyp, 'c) vval \<Rightarrow> bool"
-  where
-"\<xi>p1 f x y = (if f = ''repeat'' then vrepeatp \<xi>p0 x y else \<xi>p0 f x y)"
+section "Monomorphisation lemmas"
 
 context value_sem begin
 
@@ -46,7 +49,7 @@ lemma vrepeat_bod_monoexpr_correct:
   apply (induct n arbitrary: acc)
    apply clarsimp
   apply clarsimp
-  apply (rename_tac b)
+  apply (rename_tac n acc b)
   apply (case_tac b; clarsimp)
    apply (rule exI, rule conjI, simp)
    apply (rule_tac x = b in exI; clarsimp)
@@ -62,6 +65,7 @@ lemma vrepeat_bod_monoexpr_correct:
    apply clarsimp
    apply (rename_tac v)
    apply (case_tac v; clarsimp)
+  apply (rename_tac acc')
   apply (frule_tac \<gamma> = "[VRecord [acc, obsv]]" and
       v' = "VPrim (LBool False)" and
       e = "App (vvalfun_to_expr f) (Var 0)" and
@@ -97,375 +101,22 @@ lemma vrepeat_bod_monoexpr_correct:
   apply (intro exI conjI; assumption)
   done
 
-lemma rename_mono_prog_\<xi>m0_\<xi>p0:
-  "rename_mono_prog rename' \<Xi>' \<xi>m0 \<xi>p0"
-  unfolding rename_mono_prog_def \<xi>m0_def \<xi>p0_def
-  by clarsimp
-
-lemma vrepeat_monoexpr_correct:
+lemma prepeat_monoexpr_correct:
   "\<And>v v'.
        \<lbrakk>proc_ctx_wellformed \<Xi>';
         \<xi>' matches \<Xi>';
         rename_mono_prog rename' \<Xi>' \<xi>' \<xi>'';
         vrepeat \<Xi>' \<xi>' \<tau>a \<tau>o (rename_val rename' (monoval v)) v'\<rbrakk>
-       \<Longrightarrow> \<exists>v''. v' = rename_val rename' (monoval v'') \<and> vrepeatp \<xi>'' v v''"
-  unfolding vrepeat_def vrepeatp_def
+       \<Longrightarrow> \<exists>v''. v' = rename_val rename' (monoval v'') \<and> prepeat \<xi>'' v v''"
+  unfolding vrepeat_def prepeat_def
   apply clarsimp
+  apply (rename_tac v v' n f g acc obsv)
   apply (case_tac v; clarsimp)
+  apply (rename_tac z za zb zc zd)
   apply (case_tac z; clarsimp)
-  apply (drule_tac \<xi>'' = \<xi>'' in  vrepeat_bod_monoexpr_correct[rotated 7]; simp?)
-  done
-
-lemma rename_mono_prog_\<Xi>_\<xi>m0_\<xi>p0:
-  "rename_mono_prog rename' \<Xi>' \<xi>m0 \<xi>p0"
-  unfolding rename_mono_prog_def \<xi>m0_def \<xi>p0_def
-  by clarsimp
-
-lemma rename_mono_prog_\<Xi>_\<xi>m1_\<xi>p1:
-  "rename_mono_prog rename \<Xi> \<xi>m1 \<xi>p1"
-  unfolding rename_mono_prog_def
-  apply (clarsimp simp: \<xi>m1_def \<xi>p1_def)
-  apply (rule conjI; clarsimp)
-   apply (subst (asm) rename_def; clarsimp simp: assoc_lookup.simps split: if_splits)
-   apply (rule vrepeat_monoexpr_correct[OF _ \<xi>m0_matches_\<Xi> rename_mono_prog_\<xi>m0_\<xi>p0]; simp?)
-  apply (clarsimp simp: \<xi>m0_def)
+  apply (drule_tac \<xi>'' = \<xi>'' in vrepeat_bod_monoexpr_correct[rotated 7]; simp?)
   done
 
 end (* of context *)
-
-(*
-
-
-context value_sem begin
-definition
-  rename_mono_prog' ::
-  "(('f \<times> type list) \<Rightarrow> 'f) \<Rightarrow> ('f \<Rightarrow> poly_type) \<Rightarrow> ('f, 'a) vabsfuns \<Rightarrow> ('f, 'a) vabsfuns \<Rightarrow> bool"
-where
-  "rename_mono_prog' rename' \<Xi>' \<xi>\<^sub>r\<^sub>m \<xi>\<^sub>p \<equiv>
-     \<xi>\<^sub>r\<^sub>m matches \<Xi>' \<longrightarrow>
-     proc_ctx_wellformed \<Xi>' \<longrightarrow>
-     (\<forall>f ts v v' v''. \<xi>\<^sub>r\<^sub>m (rename' (f, ts)) (rename_val rename' (monoval v)) v'' \<longrightarrow>
-        (\<xi>\<^sub>p f v v' \<longrightarrow>  v'' = (rename_val rename' (monoval v'))) \<and> (\<exists>v'. \<xi>\<^sub>p f v v'))"
-
-lemma
-  "rename_mono_prog' rename' \<Xi>' \<xi>\<^sub>r\<^sub>m \<xi>\<^sub>p \<Longrightarrow> rename_mono_prog rename' \<Xi>' \<xi>\<^sub>r\<^sub>m \<xi>\<^sub>p"
-  unfolding rename_mono_prog_def rename_mono_prog'_def
-  apply clarsimp
-  apply (erule_tac x = f in allE)
-  apply (erule_tac x = ts in allE)
-  apply (subgoal_tac "\<exists>v'. \<xi>\<^sub>p f v v'")
-   apply (erule exE)
-   apply (erule_tac x = v in allE)
-   apply (erule_tac x = v'a in allE)
-   apply (erule_tac x = v' in allE)
-   apply clarsimp
-   apply (intro exI conjI; simp)
-  apply clarsimp
-  done
-end (* of context *)
-
-context shallow begin
-lemma repeat_bod'_monocorrect:
-  "\<lbrakk>proc_ctx_wellformed \<Xi>';
-    \<xi>' matches \<Xi>';
-    rename_mono_prog rename' \<Xi>' \<xi>' \<xi>'';
-    \<Xi>' \<turnstile> (rename_val rename' (monoval acc)) :v \<tau>a;
-    \<Xi>' \<turnstile> (rename_val rename' (monoval obsv)) :v \<tau>o;
-    is_vvalfun (rename_val rename' (monoval f));
-    is_vvalfun (rename_val rename' (monoval g));
-    repeat_bod' \<xi>' n (vvalfun_to_expr (rename_val rename' (monoval f))) 
-      (vvalfun_to_expr (rename_val rename' (monoval g))) (rename_val rename' (monoval acc))
-      (rename_val rename' (monoval obsv)) ret;
-        \<Xi>', [], [option.Some (TRecord [(''acc'', bang \<tau>a, Present), (''obsv'', \<tau>o, Present)] Unboxed)] 
-      \<turnstile> (App (vvalfun_to_expr (rename_val rename' (monoval f))) (Var 0)) : TPrim Bool;
-    \<Xi>', [], [option.Some (TRecord [(''acc'', \<tau>a, Present), (''obsv'', \<tau>o, Present)] Unboxed)] 
-      \<turnstile> (App (vvalfun_to_expr (rename_val rename' (monoval g))) (Var 0)) : \<tau>a\<rbrakk>
-  \<Longrightarrow> is_vvalfun f \<and> is_vvalfun g \<and> (\<exists>ret'. ret = rename_val rename' (monoval ret') \<and>
-         repeat_bod' \<xi>'' n (vvalfun_to_expr f) (vvalfun_to_expr g) acc obsv ret')"
-  oops
-
-lemma rename_monoexpr_correct':
-  assumes "proc_ctx_wellformed \<Xi>'"
-  and     "\<xi>\<^sub>r\<^sub>m matches \<Xi>'"
-  and     "rename_mono_prog' rename' \<Xi>' \<xi>\<^sub>r\<^sub>m \<xi>\<^sub>p"
-  and     "\<Xi>' \<turnstile> map (rename_val rename' \<circ> monoval) \<gamma> matches \<Gamma>"
-  shows   "\<xi>\<^sub>r\<^sub>m, map (rename_val rename' \<circ> monoval) \<gamma> \<turnstile> rename_expr rename' (monoexpr e) \<Down> v' \<Longrightarrow>
-             \<Xi>', [], \<Gamma> \<turnstile> rename_expr rename' (monoexpr e) : \<tau>  \<Longrightarrow>
-              \<xi>\<^sub>p, \<gamma> \<turnstile> e \<Down>  v \<Longrightarrow>
-              v' = rename_val rename' (monoval v)"
-  and     "\<xi>\<^sub>r\<^sub>m, map (rename_val rename' \<circ> monoval) \<gamma> \<turnstile>* map (rename_expr rename' \<circ> monoexpr) es \<Down> vs' \<Longrightarrow>
-             \<Xi>', [], \<Gamma> \<turnstile>* map (rename_expr rename' \<circ> monoexpr) es : \<tau>s \<Longrightarrow>
-             (\<xi>\<^sub>p , \<gamma> \<turnstile>* es \<Down> vs) \<Longrightarrow>
-             vs' = (map (rename_val rename' \<circ> monoval) vs)"
-  using assms
-  proof (induct \<xi>\<^sub>r\<^sub>m "map (rename_val rename' \<circ> monoval) \<gamma>" "rename_expr rename' (monoexpr e)" v'
-            and \<xi>\<^sub>r\<^sub>m "map (rename_val rename' \<circ> monoval) \<gamma>" "map (rename_expr rename' \<circ> monoexpr) es" vs'
-         arbitrary: \<tau> \<Gamma> \<gamma> e v
-           and \<tau>s \<Gamma> \<gamma> es vs
-         rule: v_sem_v_sem_all.inducts)
-    case (v_sem_var \<xi> i)
-    then show ?case
-      by (cases e) (force intro: v_sem_v_sem_all.v_sem_var dest: matches_length)+
-  next
-    case (v_sem_lit \<xi> l)
-    then show ?case 
-      apply (cases e; clarsimp intro: v_sem_v_sem_all.v_sem_lit)
-      apply (erule v_sem_litE; clarsimp)
-      done
-  next
-    case (v_sem_prim \<xi> as as' p)
-    then show ?case
-      apply (cases e; clarsimp intro: v_sem_v_sem_all.v_sem_lit)
-      apply (erule v_sem_primE; clarsimp)
-      apply (erule typing_primE; clarsimp)
-      apply (drule_tac x = \<gamma> in meta_spec)
-      apply (rename_tac e' bs ts t)
-      apply (drule_tac x = e' and y = \<Gamma> in meta_spec2; clarsimp)
-      apply (drule_tac x = "map TPrim ts" and y = bs in meta_spec2; clarsimp)
-      apply (frule(4) preservation(2) [where \<tau>s = "[]" and K = "[]", simplified])
-      apply (frule v_t_map_TPrimD)
-      apply clarsimp
-      apply (frule eval_prim_preservation)
-       apply simp
-      apply (erule vval_typing.cases, simp_all)
-      apply (drule map_rename_monoval_prim_prim)
-      apply clarsimp
-      done
-  next
-    case (v_sem_fun \<xi> f ts)
-    then show ?case 
-      by (cases e) (auto intro: v_sem_v_sem_all.v_sem_fun)
-  next
-    case (v_sem_afun \<xi> f ts)
-    then show ?case
-      by (cases e) (auto intro: v_sem_v_sem_all.v_sem_afun)
-  next
-    case (v_sem_abs_app \<xi> x f ts y a r)
-    then show ?case
-      apply (cases e; clarsimp intro: v_sem_v_sem_all.v_sem_con)
-      apply (rename_tac b c)
-      apply (drule_tac x = \<gamma> in meta_spec)
-      apply (drule_tac x = \<gamma> in meta_spec)
-      apply (erule typing_appE; clarsimp)
-      apply (drule_tac x = b in meta_spec)
-      apply (drule_tac x = c in meta_spec)
-      apply clarsimp
-      apply (rename_tac \<Gamma>1 \<Gamma>2 t)
-      apply (drule_tac x = \<Gamma>1 and y = "TFun t \<tau>" in meta_spec2)
-      apply (drule_tac x = \<Gamma>2 and y = t in meta_spec2)
-      apply clarsimp
-      apply (frule matches_split'(1); simp?)
-      apply (frule matches_split'(2); simp?)
-      apply (erule v_sem_appE)
-       apply (rename_tac f' ts' a')
-       apply (drule_tac x = "VAFunction f' ts'" in meta_spec)
-       apply (drule_tac x = a' in meta_spec)
-       apply (clarsimp simp: rename_mono_prog'_def)
-      apply (rename_tac f' ts' a')
-      apply (drule_tac x = "VFunction f' ts'" in meta_spec)
-      apply (drule_tac x = a' in meta_spec)
-      apply clarsimp
-      done
-  next
-    case (v_sem_cast \<xi> e l \<tau> l')
-    then show ?case
-      apply (cases e; clarsimp intro: v_sem_v_sem_all.v_sem_con)
-      apply (erule v_sem_castE; clarsimp)
-      apply (erule typing_castE; clarsimp)
-      apply (rename_tac e' l' l'' \<tau>)
-      apply (drule_tac x = \<gamma> and y = e' in meta_spec2; clarsimp)
-      apply (rename_tac e' y y' \<tau>)
-      apply (drule_tac x = \<Gamma> and y = "TPrim (Num \<tau>)" in meta_spec2; clarsimp)
-      apply (drule_tac x = "VPrim y" in meta_spec; clarsimp)
-      done
-  next
-    case (v_sem_app \<xi> re f ts e' rv rsv \<gamma> e \<tau> \<Gamma>)
-    then show ?case
-     apply (cases e; clarsimp intro: v_sem_v_sem_all.v_sem_con)
-      apply (rename_tac b c)
-      apply (drule_tac x = \<gamma> in meta_spec)
-      apply (drule_tac x = \<gamma> in meta_spec)
-      apply (erule typing_appE; clarsimp)
-      apply (drule_tac x = b in meta_spec)
-      apply (drule_tac x = c in meta_spec)
-      apply clarsimp
-      apply (rename_tac \<Gamma>1 \<Gamma>2 t)
-      apply (drule_tac x = \<Gamma>1 and y = "TFun t \<tau>" in meta_spec2)
-      apply (drule_tac x = \<Gamma>2 and y = t in meta_spec2)
-      apply clarsimp
-      apply (frule matches_split'(1); simp?)
-      apply (frule matches_split'(2); simp?)
-      apply (erule v_sem_appE)
-       apply (rename_tac f' ts' a')
-       apply (drule_tac x = "VAFunction f' ts'" in meta_spec)
-       apply (drule_tac x = a' in meta_spec)
-       apply clarsimp
-      apply (rename_tac f' ts' a')
-      apply (drule_tac x = "VFunction f' ts'" in meta_spec)
-      apply (drule_tac x = a' in meta_spec)
-      apply clarsimp
-      apply (drule_tac x = "[a']" in meta_spec; simp)
-      apply (drule_tac x = "specialise ts' f'" in meta_spec; simp)
-      apply (frule(5) preservation(1) [where \<tau>s = "[]" and K = "[]", OF _ _ matches_split'(1), simplified])
-      apply (frule(5) preservation(1) [where \<tau>s = "[]" and K = "[]", OF _ _ matches_split'(2), simplified])
-      apply (erule v_t_funE; clarsimp)
-      apply (subst (asm) subtyping_simps; clarsimp)
-      apply (drule value_subtyping(1)[rotated 1]; simp?)
-      apply (rename_tac  ta u t')
-      apply (drule_tac x = "[Some ta]" and y = u in meta_spec2; clarsimp)
-      apply (drule_tac x = v in meta_spec; clarsimp)
-      apply (drule meta_mp; simp add: matches_def)
-      done
-  next
-    case (v_sem_con \<xi> x x' uu t)
-    then show ?case
-      apply (cases e; clarsimp intro: v_sem_v_sem_all.v_sem_con)
-      apply (erule v_sem_conE; clarsimp)
-      apply (erule typing_conE; clarsimp)
-      done
-  next
-    case (v_sem_member \<xi> e fs f)
-    then show ?case 
-      apply (cases e; clarsimp intro: v_sem_v_sem_all.v_sem_member)
-      apply (erule v_sem_memberE; clarsimp)
-      apply (erule typing_memberE; clarsimp)
-      apply (elim meta_allE meta_impE; simp?)
-      apply (frule(4) preservation [where \<tau>s = "[]" and K = "[]", simplified])
-      apply (erule v_t_recordE)
-      apply (frule vval_typing_record_length)
-      apply clarsimp
-      done
-  next
-    case (v_sem_unit \<xi>)
-    then show ?case
-      apply (cases e; clarsimp intro!:  v_sem_v_sem_all.v_sem_unit)
-      apply (erule v_sem_unitE; clarsimp)
-      done
-  next
-    case (v_sem_tuple \<xi> x x' y y')
-    then show ?case
-      apply (cases e; clarsimp intro!:  v_sem_v_sem_all.v_sem_tuple matches_split')
-      apply (erule v_sem_tupleE; clarsimp)
-      apply (erule typing_tupleE)
-      apply (frule  matches_split'(1); simp?)
-      apply (frule  matches_split'(2); simp?)
-      apply clarsimp
-      done
-  next
-    case (v_sem_esac \<xi> t ts v)
-    then show ?case
-      apply (cases e; clarsimp intro!:  v_sem_v_sem_all.v_sem_esac)
-      apply (erule v_sem_esacE)
-      apply (erule typing_esacE)
-      apply (rename_tac e' ts')
-      apply clarsimp
-      apply (elim meta_allE meta_impE; simp?)
-      apply clarsimp
-      done
-  next
-    case (v_sem_let \<xi> a a' b b')
-    then show ?case 
-      apply (cases e; clarsimp intro!:  v_sem_v_sem_all.v_sem_let)
-      apply (erule v_sem_letE)
-      apply (erule typing_letE)
-      apply (frule matches_split'(1); simp?)
-      apply (frule matches_split'(2); simp?)
-      apply (rename_tac e1 e2 aa \<Gamma>1 \<Gamma>2 t)
-      apply (drule_tac x = \<gamma> and y = e1 in meta_spec2; clarsimp)
-      apply (drule_tac x = \<Gamma>1 and y = t in meta_spec2; clarsimp)
-      apply (drule_tac x = aa in meta_spec; clarsimp)
-      apply (drule_tac x = "aa # \<gamma>" and y = e2 in meta_spec2; clarsimp)
-      apply (drule_tac x = "Some t # \<Gamma>2" and y = \<tau> in meta_spec2; clarsimp)
-      apply (drule_tac x = v in meta_spec; clarsimp)
-      apply (frule(4) preservation [where \<tau>s = "[]" and K = "[]", simplified])
-      apply (drule(2) matches_cons'[OF matches_split'(2)])
-      apply clarsimp
-      done
-  next
-    case (v_sem_letbang \<xi> a a' b b' vs)
-    then show ?case
-      apply (cases e; clarsimp intro!:  v_sem_v_sem_all.v_sem_letbang)
-      apply (erule v_sem_letBangE)
-      apply (erule typing_letbE)
-      apply (frule matches_split_bang'(1); simp?)
-      apply (frule matches_split_bang'(2); simp?)
-      apply (rename_tac e1 e2 aa \<Gamma>1 \<Gamma>2 t k)
-      apply (drule_tac x = \<gamma> and y = e1 in meta_spec2; clarsimp)
-      apply (drule_tac x = \<Gamma>1 and y = t in meta_spec2; clarsimp)
-      apply (drule_tac x = aa in meta_spec; clarsimp)
-      apply (drule_tac x = "aa # \<gamma>" and y = e2 in meta_spec2; clarsimp)
-      apply (drule_tac x = "Some t # \<Gamma>2" and y = \<tau> in meta_spec2; clarsimp)
-      apply (drule_tac x = v in meta_spec; clarsimp)
-      apply (frule(4) preservation [where \<tau>s = "[]" and K = "[]", simplified])
-      apply (drule(2) matches_cons'[OF matches_split_bang'(2)])
-      apply clarsimp
-      done
-  next
-    case (v_sem_case_m \<xi> x t v m m' n)
-    then show ?case sorry
-  next
-    case (v_sem_case_nm \<xi> x t' v t n n' m)
-    then show ?case sorry
-  next
-    case (v_sem_if \<xi> x b t e r)
-    then show ?case sorry
-  next
-    case (v_sem_struct \<xi> xs vs ts)
-    then show ?case
-      apply (cases e; clarsimp intro: v_sem_v_sem_all.v_sem_struct)
-      apply (erule v_sem_structE; clarsimp)
-      apply (erule typing_structE; clarsimp)
-      done
-  next
-    case (v_sem_take \<xi> x fs f e e')
-    then show ?case sorry
-  next
-    case (v_sem_put \<xi> x fs e e' f)
-    then show ?case sorry
-  next
-    case (v_sem_split \<xi> x a b e e')
-    then show ?case
-      apply(cases e; clarsimp intro!: v_sem_v_sem_all.v_sem_split)
-      apply (erule v_sem_splitE)
-      apply (erule typing_splitE)
-      apply (frule matches_split'(1); simp?)
-      apply (frule matches_split'(2); simp?)
-      apply (rename_tac e1 e2 aa bb \<Gamma>1 \<Gamma>2 t u)
-      apply (drule_tac x = \<gamma> and y = e1 in meta_spec2; clarsimp)
-      apply (drule_tac x = \<Gamma>1 and y = "TProduct t u" in meta_spec2; clarsimp)
-      apply (drule_tac x = "VProduct aa bb"  in meta_spec; clarsimp)
-      apply (drule_tac x = "aa # bb # \<gamma>" and y = e2 in meta_spec2; clarsimp)
-      apply (drule_tac x = "Some t # Some u # \<Gamma>2" and y = \<tau> in meta_spec2; clarsimp)
-      apply (drule_tac x = v in meta_spec; clarsimp)
-      apply (frule(5) preservation [where \<tau>s = "[]" and K = "[]", OF _ _ matches_split'(1), simplified])
-      apply (erule v_t_productE; clarsimp)
-      apply (rename_tac t u)
-      apply (drule_tac x = "rename_val rename' (monoval bb)" and ?\<Gamma> = \<Gamma>2 in matches_cons'; simp?)
-      apply (drule_tac x = "rename_val rename' (monoval aa)" and ?\<Gamma> = "Some u # \<Gamma>2" in matches_cons'; simp?)
-      apply clarsimp
-      done
-  next
-    case (v_sem_promote \<xi> e e' t')
-    then show ?case
-      apply(cases e; clarsimp intro!: v_sem_v_sem_all.v_sem_promote)
-      apply (erule v_sem_promoteE)
-      apply (erule typing_promoteE)
-      apply clarsimp
-      done
-  next
-    case (v_sem_all_empty \<xi>)
-    then show ?case
-      by (cases e) (fastforce intro: v_sem_v_sem_all.v_sem_all_empty elim: v_sem_all_NilE)+
-  next
-    case (v_sem_all_cons \<xi> x v xs vs)
-    then show ?case
-      apply (cases e;clarsimp intro!: v_sem_v_sem_all.intros)
-      apply (elim v_sem_all_ConsE typing_all_consE; clarsimp; frule matches_split'(1); simp?; frule matches_split'(2); simp?; clarsimp)+
-      done
-  qed
-
-end (* of context *)
-*)
-
 
 end
