cogent/examples/repeat/CogentTypingHelper.thy
@@ -1,0 +1,73 @@
+theory CogentTypingHelper
+  imports Type_Proof.TypeTrackingTyping
+begin
+
+section "Typing helpers"
+
+subsection "Cogent functions"
+
+lemma typing_mono_app_cogent_fun:
+  "\<Xi>', [], [option.Some a] \<turnstile> f : b \<Longrightarrow> \<Xi>', [], [option.Some a] \<turnstile> App (Fun f []) (Var 0) : b"
+  apply (frule typing_to_kinding_env(1); simp?)
+  apply (rule typing_app[where x = a and y = b and ?\<Gamma>1.0 = "[option.None]" and ?\<Gamma>2.0 = "[option.Some a]"]; simp?)
+    apply (clarsimp simp: split_conv_all_nth)
+    apply (rule right; simp)
+    apply (rule typing_fun[where ts = "[]", OF _ _ _ _]; (simp add: Cogent.empty_def weakening_conv_all_nth)?)
+   apply (rule none)
+  apply (rule typing_var; simp add: Cogent.empty_def weakening_conv_all_nth)
+  apply (rule keep; simp)
+  done
+
+lemma typing_mono_fun_cogent_fun:
+  "\<Xi>', [], [option.Some a] \<turnstile> f : b \<Longrightarrow> \<Xi>', [], [option.None] \<turnstile> Fun f [] : TFun a b"
+  apply (frule typing_to_kinding_env(1); simp?)
+  apply (rule typing_fun[where ts = "[]", OF _ _ _ _]; (simp add: Cogent.empty_def weakening_conv_all_nth)?)
+  apply (rule none)
+  done
+
+lemma typing_mono_fun_imp_appfun:
+  "\<Xi>', [], [option.None] \<turnstile> Fun f [] : TFun a b \<Longrightarrow> \<Xi>', [], [option.Some a] \<turnstile> App (Fun f []) (Var 0) : b"
+  apply (frule typing_to_wellformed(1))
+  apply (rule typing_app[where x = a and y = b and ?\<Gamma>1.0 = "[option.None]" and ?\<Gamma>2.0 = "[option.Some a]"]; simp?)
+   apply (clarsimp simp: split_conv_all_nth)
+   apply (rule right; simp)
+  apply (rule typing_var; simp add: Cogent.empty_def weakening_conv_all_nth)
+  apply (rule keep; simp)
+  done
+
+subsection "Abstract functions"
+
+lemma typing_mono_app_cogent_absfun:
+  "\<lbrakk>proc_ctx_wellformed \<Xi>'; \<Xi>' f = ([], a, b)\<rbrakk> \<Longrightarrow> \<Xi>', [], [option.Some a] \<turnstile> App (AFun f []) (Var 0) : b"
+  apply (unfold  proc_ctx_wellformed_def)
+  apply (erule_tac x = f in allE; clarsimp)
+  apply (rule typing_app[where x = a and y = b and ?\<Gamma>1.0 = "[option.None]" and ?\<Gamma>2.0 = "[option.Some a]"]; simp?)
+    apply (clarsimp simp: split_conv_all_nth)
+    apply (rule right; simp)
+   apply (rule typing_afun[where ts = "[]", OF _ _ _ _]; (simp add: Cogent.empty_def weakening_conv_all_nth)?)
+    apply clarsimp
+   apply (rule none)
+  apply (rule typing_var; simp add: Cogent.empty_def weakening_conv_all_nth)
+  apply (rule keep; simp)
+  done
+
+lemma typing_mono_afun_cogent_absfun:
+  "\<lbrakk>proc_ctx_wellformed \<Xi>'; \<Xi>' f = ([], a, b)\<rbrakk> \<Longrightarrow> \<Xi>', [], [option.None] \<turnstile> AFun f [] : TFun a b"
+  apply (unfold  proc_ctx_wellformed_def)
+  apply (erule_tac x = f in allE; clarsimp)
+  apply (rule typing_afun[where ts = "[]", OF _ _ _ _]; (simp add: Cogent.empty_def weakening_conv_all_nth)?)
+   apply clarsimp
+  apply (rule none)
+  done
+
+lemma typing_mono_afun_imp_appafun:
+  "\<Xi>', [], [option.None] \<turnstile> AFun f [] : TFun a b \<Longrightarrow> \<Xi>', [], [option.Some a] \<turnstile> App (AFun f []) (Var 0) : b"
+  apply (frule typing_to_wellformed(1))
+  apply (rule typing_app[where x = a and y = b and ?\<Gamma>1.0 = "[option.None]" and ?\<Gamma>2.0 = "[option.Some a]"]; simp?)
+   apply (clarsimp simp: split_conv_all_nth)
+   apply (rule right; simp)
+  apply (rule typing_var; simp add: Cogent.empty_def weakening_conv_all_nth)
+  apply (rule keep; simp)
+  done
+
+end
