cogent/examples/repeat/RepeatCorrespondence.thy
@@ -1,10 +1,10 @@
 theory RepeatCorrespondence
-  imports RepeatUpdate RepeatValue
+  imports RepeatUpdate RepeatValue CorrespondenceHelper
 begin
 
 context correspondence begin
 
-inductive_cases u_v_primE'     [elim] : "\<Xi>', \<sigma> \<turnstile> UPrim l \<sim> x : TPrim \<tau> \<langle>r, w\<rangle>"
+section "Mono-correspondence"
 
 lemma uvrepeat_bod_monocorrespondence:
   "\<lbrakk>proc_ctx_wellformed \<Xi>';
@@ -23,6 +23,7 @@ lemma uvrepeat_bod_monocorrespondence:
     apply blast
    apply (rule upd.frame_id)
   apply clarsimp
+  apply (rename_tac n \<sigma> uacc ra wa vacc b ba)
   apply (case_tac b; clarsimp)
    apply (drule_tac r = "(ra \<union> wa) \<union> ro"  and w = "{}" in mono_correspondence(1)[rotated 3]; simp?)
     apply (intro u_v_matches_some[where r' = "{}" and w' = "{}", simplified]
@@ -67,7 +68,9 @@ lemma uvrepeat_bod_monocorrespondence:
   apply (erule upd.frame_trans; assumption)
   done
 
-lemma uvrepeat_bod_val_executes_from_upd_executes:
+section "Upward propagation"
+
+lemma uvrepeat_bod_upward_propagation:
   "\<lbrakk>proc_ctx_wellformed \<Xi>';
     \<xi>u \<sim> \<xi>v matches-u-v \<Xi>';
     \<Xi>', \<sigma> \<turnstile> uacc \<sim> vacc : \<tau>a \<langle>ra, wa\<rangle>;
@@ -81,6 +84,7 @@ lemma uvrepeat_bod_val_executes_from_upd_executes:
    apply clarsimp
    apply (intro exI; simp)
   apply clarsimp
+  apply (rename_tac n \<sigma> uacc ra wa vacc b)
   apply (case_tac b; clarsimp)
    apply (rule_tac x = vacc in exI)
    apply clarsimp
@@ -105,7 +109,7 @@ lemma uvrepeat_bod_val_executes_from_upd_executes:
                   u_v_r_empty; simp?)
     apply (rule upd_val_rel_bang(1); simp)
    apply clarsimp
-   apply (erule u_v_primE'; clarsimp)
+   apply (erule u_v_uprimE; clarsimp)
   apply (frule_tac r = "(ra \<union> wa) \<union> ro"  and w = "{}" and
       \<gamma>' = "[VRecord [vacc, vobsv]]" in val_executes_from_upd_executes(1)[rotated 3]; simp?)
     apply (intro u_v_matches_some[where r' = "{}" and w' = "{}", simplified]
@@ -125,7 +129,7 @@ lemma uvrepeat_bod_val_executes_from_upd_executes:
                   u_v_r_empty; simp?)
    apply (rule upd_val_rel_bang(1); simp)
   apply clarsimp
-  apply (erule u_v_primE'; clarsimp)
+  apply (erule u_v_uprimE; clarsimp)
   apply (thin_tac "upd.frame _ {} _ {}")
   apply (frule_tac r = "ra \<union> ro"  and w = wa and
       \<gamma>' = "[VRecord [vacc, vobsv]]" and
@@ -160,6 +164,8 @@ lemma uvrepeat_bod_val_executes_from_upd_executes:
   apply clarsimp
   apply (intro exI conjI; assumption)
   done
+
+section "Mono-correspondence and upward propagation"
 
 lemma uvrepeat_monocorrespond_upward_propagation:
   "\<And>\<sigma> \<sigma>' au av v v' r w.
@@ -198,7 +204,7 @@ lemma uvrepeat_monocorrespond_upward_propagation:
     apply blast
    apply blast
   apply (drule_tac vacc = acc' and vobsv = obsv' and ra = ra and wa = wa
-      in uvrepeat_bod_val_executes_from_upd_executes[rotated 5]; simp?)
+      in uvrepeat_bod_upward_propagation[rotated 5]; simp?)
    apply blast
   apply (erule u_v_tfunE; clarsimp)+
     apply (intro conjI exI upd_val_rel_to_vval_typing(1); assumption)+
@@ -208,224 +214,4 @@ lemma uvrepeat_monocorrespond_upward_propagation:
 
 end (* of context *)
 
-context correspondence_init begin
-
-lemma \<xi>_0_\<xi>m0_matchesuv_\<Xi>:
-  "\<xi>_0 \<sim> val.\<xi>m0 matches-u-v \<Xi>'"
-  unfolding proc_env_u_v_matches_def \<xi>0_def val.\<xi>m0_def
-  by clarsimp
-
-lemma \<xi>_1_\<xi>m1_matchesuv_\<Xi>:
-  "\<xi>_1 \<sim> val.\<xi>m1 matches-u-v \<Xi>"
-  unfolding proc_env_u_v_matches_def \<xi>1_def val.\<xi>m1_def
-  apply clarsimp
-  apply (rule conjI; clarsimp)
-  apply (subst (asm) \<Xi>_def; clarsimp simp: repeat_0_type_def)
-   apply (rule uvrepeat_monocorrespond_upward_propagation[OF proc_ctx_wellformed_\<Xi> \<xi>_0_\<xi>m0_matchesuv_\<Xi>];
-      (simp add: abbreviated_type_defs)?)
-  apply (clarsimp simp: \<xi>0_def val.\<xi>m0_def)
-  done
-
-end (* of context *)
-(*
-lemma repeat_bod_monocorrespondence:
-  "\<lbrakk>proc_ctx_wellformed \<Xi>';
-    \<xi>u \<sim> \<xi>v matches-u-v \<Xi>';
-    \<Xi>', \<sigma> \<turnstile> uacc \<sim> vacc : \<tau>a \<langle>ra, wa\<rangle>;
-    \<Xi>', \<sigma> \<turnstile> uobsv \<sim> vobsv : \<tau>o \<langle>ro, {}\<rangle>;
-    ro \<inter> wa = {};
-    repeat_bod \<xi>u n f g \<sigma> \<sigma>' \<tau>a uacc \<tau>o uobsv uret;
-    repeat_bod' \<xi>v n f g vacc vobsv vret;
-    \<Xi>', [], [option.Some (TRecord [(''acc'', bang \<tau>a, Present), (''obsv'', \<tau>o, Present)] Unboxed)] \<turnstile> (App f (Var 0)) : TPrim Bool;
-    \<Xi>', [], [option.Some (TRecord [(''acc'', \<tau>a, Present), (''obsv'', \<tau>o, Present)] Unboxed)] \<turnstile> (App g (Var 0)) : \<tau>a\<rbrakk>
-      \<Longrightarrow>\<exists>r' w'.  \<Xi>', \<sigma>' \<turnstile> uret \<sim> vret : \<tau>a \<langle>r', w'\<rangle> \<and> r' \<subseteq> (ra \<union> ro) \<and> upd.frame \<sigma> wa \<sigma>' w'"
-  apply (induct n arbitrary: \<sigma> uacc ra wa vacc)
-   apply clarsimp
-   apply (intro exI conjI; simp?)
-    apply blast
-   apply (rule upd.frame_id)
-  apply (clarsimp split: if_splits)
-     apply (intro exI conjI; simp?)
-      apply blast
-     apply (rule upd.frame_id)
-    apply (rule FalseE)
-    apply (drule_tac r = "(ra \<union> wa) \<union> ro"  and w = "{}" in mono_correspondence(1)[rotated 3]; simp?)
-     apply (intro u_v_matches_some[where r' = "{}" and w' = "{}", simplified]
-                  u_v_matches_empty[where \<tau>s = "[]", simplified]
-                  u_v_struct
-                  u_v_r_cons1[where w' = "{}", simplified]
-                  u_v_r_cons1[where r' = "{}" and w' = "{}", simplified]
-                  u_v_r_empty; simp?)
-     apply (rule upd_val_rel_bang(1); simp)
-    apply clarsimp
-    apply (erule u_v_primE; clarsimp)
-   apply (rule FalseE)
-   apply (drule_tac r = "(ra \<union> wa) \<union> ro"  and w = "{}" in mono_correspondence(1)[rotated 3]; simp?)
-    apply (intro u_v_matches_some[where r' = "{}" and w' = "{}", simplified]
-                 u_v_matches_empty[where \<tau>s = "[]", simplified]
-                 u_v_struct
-                 u_v_r_cons1[where w' = "{}", simplified]
-                 u_v_r_cons1[where r' = "{}" and w' = "{}", simplified]
-                 u_v_r_empty; simp?)
-    apply (rule upd_val_rel_bang(1); simp)
-   apply clarsimp
-   apply (erule u_v_primE; clarsimp)
-  apply (rename_tac \<sigma>'' uacc' vacc')
-  apply (drule_tac r = "ra \<union> ro"  and w = wa and 
-      \<gamma> = "[URecord [(uacc, type_repr \<tau>a), (uobsv, type_repr \<tau>o)]]" in mono_correspondence(1)[rotated 3]; simp?)
-   apply (intro u_v_matches_some[where r' = "{}" and w' = "{}", simplified]
-                u_v_matches_empty[where \<tau>s = "[]", simplified]
-                u_v_struct
-                u_v_r_cons1[where w' = "{}", simplified]
-                u_v_r_cons1[where r' = "{}" and w' = "{}", simplified]
-                u_v_r_empty; simp?)
-   apply blast
-  apply clarsimp
-  apply (rename_tac r' w')
-  apply (frule_tac u = uobsv and v = vobsv in upd_val_rel_frame(1)[rotated 3]; simp?; clarsimp?)
-   apply (frule_tac v = uobsv and v' = vobsv in frame_noalias_upd_val_rel'(2); simp?; clarsimp?)
-  apply (elim meta_allE meta_impE, assumption, assumption, assumption, assumption, assumption)
-  apply clarsimp
-  apply (intro exI conjI, assumption, blast)
-  apply (erule upd.frame_trans; assumption)
-  done
-
-
-
-lemma repeat_bod_val_executes_from_upd_executes:
-  "\<lbrakk>proc_ctx_wellformed \<Xi>';
-    \<xi>u \<sim> \<xi>v matches-u-v \<Xi>';
-    \<Xi>', \<sigma> \<turnstile> uacc \<sim> vacc : \<tau>a \<langle>ra, wa\<rangle>;
-    \<Xi>', \<sigma> \<turnstile> uobsv \<sim> vobsv : \<tau>o \<langle>ro, {}\<rangle>;
-    ro \<inter> wa = {};
-    repeat_bod \<xi>u n f g \<sigma> \<sigma>' \<tau>a uacc \<tau>o uobsv uret;
-    \<Xi>', [], [option.Some (TRecord [(''acc'', bang \<tau>a, Present), (''obsv'', \<tau>o, Present)] Unboxed)] \<turnstile> (App f (Var 0)) : TPrim Bool;
-    \<Xi>', [], [option.Some (TRecord [(''acc'', \<tau>a, Present), (''obsv'', \<tau>o, Present)] Unboxed)] \<turnstile> (App g (Var 0)) : \<tau>a\<rbrakk>
-      \<Longrightarrow> \<exists>vret. repeat_bod' \<xi>v n f g vacc vobsv vret"
-  apply (induct n arbitrary: \<sigma> uacc ra wa vacc)
-   apply clarsimp
-   apply (rule_tac x = vacc in exI)
-   apply clarsimp
-  apply (clarsimp split: if_splits)
-   apply (rule_tac x = vacc in exI)
-   apply clarsimp
-   apply (rule conjI; clarsimp)
-    apply (rule FalseE)
-    apply (drule_tac r = "(ra \<union> wa) \<union> ro"  and w = "{}" in mono_correspondence(1)[rotated 3]; simp?)
-     apply (intro u_v_matches_some[where r' = "{}" and w' = "{}", simplified]
-                  u_v_matches_empty[where \<tau>s = "[]", simplified]
-                  u_v_struct
-                  u_v_r_cons1[where w' = "{}", simplified]
-                  u_v_r_cons1[where r' = "{}" and w' = "{}", simplified]
-                  u_v_r_empty; simp?)
-     apply (rule upd_val_rel_bang(1); simp)
-    apply clarsimp
-    apply (erule u_v_primE; clarsimp)
-   apply (frule_tac r = "(ra \<union> wa) \<union> ro"  and w = "{}" and
-      \<gamma>' = "[VRecord [vacc, vobsv]]" in val_executes_from_upd_executes(1)[rotated 3]; simp?)
-     apply (intro u_v_matches_some[where r' = "{}" and w' = "{}", simplified]
-                  u_v_matches_empty[where \<tau>s = "[]", simplified]
-                  u_v_struct
-                  u_v_r_cons1[where w' = "{}", simplified]
-                  u_v_r_cons1[where r' = "{}" and w' = "{}", simplified]
-                  u_v_r_empty; simp?)
-     apply (rule upd_val_rel_bang(1); simp)
-   apply clarsimp
-    apply (frule_tac r = "(ra \<union> wa) \<union> ro"  and w = "{}" in mono_correspondence(1)[rotated 3]; simp?)
-     apply (intro u_v_matches_some[where r' = "{}" and w' = "{}", simplified]
-                  u_v_matches_empty[where \<tau>s = "[]", simplified]
-                  u_v_struct
-                  u_v_r_cons1[where w' = "{}", simplified]
-                  u_v_r_cons1[where r' = "{}" and w' = "{}", simplified]
-                  u_v_r_empty; simp?)
-     apply (rule upd_val_rel_bang(1); simp)
-    apply clarsimp
-   apply (erule u_v_primE'; clarsimp)
-    apply (frule_tac r = "(ra \<union> wa) \<union> ro"  and w = "{}" and v' = "VPrim (LBool False)" in mono_correspondence(1)[rotated 3]; simp?)
-     apply (intro u_v_matches_some[where r' = "{}" and w' = "{}", simplified]
-                  u_v_matches_empty[where \<tau>s = "[]", simplified]
-                  u_v_struct
-                  u_v_r_cons1[where w' = "{}", simplified]
-                  u_v_r_cons1[where r' = "{}" and w' = "{}", simplified]
-                  u_v_r_empty; simp?)
-     apply (rule upd_val_rel_bang(1); simp)
-   apply clarsimp
-   apply (erule u_v_primE; clarsimp)
-  apply (frule_tac r = "ra \<union> ro"  and w = wa and
-      \<gamma>' = "[VRecord [vacc, vobsv]]" and
-      e = "App g (Var 0)" in val_executes_from_upd_executes(1)[rotated 3]; simp?)
-   apply (intro u_v_matches_some[where r' = "{}" and w' = "{}", simplified]
-                  u_v_matches_empty[where \<tau>s = "[]", simplified]
-                  u_v_struct
-                  u_v_r_cons1[where w' = "{}", simplified]
-                  u_v_r_cons1[where r' = "{}" and w' = "{}", simplified]
-                  u_v_r_empty; simp?)
-   apply blast
-  apply clarsimp
-  apply (frule_tac r = "ra \<union> ro"  and w = wa and
-      \<gamma>' = "[VRecord [vacc, vobsv]]" and
-      e = "App g (Var 0)" in mono_correspondence(1)[rotated 3]; simp?)
-   apply (intro u_v_matches_some[where r' = "{}" and w' = "{}", simplified]
-                  u_v_matches_empty[where \<tau>s = "[]", simplified]
-                  u_v_struct
-                  u_v_r_cons1[where w' = "{}", simplified]
-                  u_v_r_cons1[where r' = "{}" and w' = "{}", simplified]
-                  u_v_r_empty; simp?)
-   apply blast
-  apply clarsimp
-  apply (rename_tac  \<sigma>'' uacc' vacc' r' w')
-  apply (frule_tac u = uobsv and v = vobsv in upd_val_rel_frame(1)[rotated 3]; simp?; clarsimp?)
-  apply (frule_tac v = uobsv and v' = vobsv in frame_noalias_upd_val_rel'(2); simp?; clarsimp?)
-  apply (elim meta_allE meta_impE, assumption, assumption, assumption, assumption)
-  apply clarsimp
-  apply (rename_tac vret)
-  apply (rule_tac x = vret in exI)
-  apply clarsimp
-  apply (rule conjI; clarsimp)
-   apply (intro exI conjI; assumption)
-  apply (rule conjI)
-   apply clarsimp
-   apply (rule FalseE)
-   apply (frule_tac r = "(ra \<union> wa) \<union> ro"  and w = "{}" in mono_correspondence(1)[rotated 3]; simp?)
-    apply (intro u_v_matches_some[where r' = "{}" and w' = "{}", simplified]
-                  u_v_matches_empty[where \<tau>s = "[]", simplified]
-                  u_v_struct
-                  u_v_r_cons1[where w' = "{}", simplified]
-                  u_v_r_cons1[where r' = "{}" and w' = "{}", simplified]
-                  u_v_r_empty; simp?)
-    apply (rule upd_val_rel_bang(1); simp)
-   apply clarsimp
-   apply (erule u_v_primE'; clarsimp)
-  apply (frule_tac r = "(ra \<union> wa) \<union> ro"  and w = "{}" and
-      \<gamma>' = "[VRecord [vacc, vobsv]]" in val_executes_from_upd_executes(1)[rotated 3]; simp?)
-   apply (intro u_v_matches_some[where r' = "{}" and w' = "{}", simplified]
-                  u_v_matches_empty[where \<tau>s = "[]", simplified]
-                  u_v_struct
-                  u_v_r_cons1[where w' = "{}", simplified]
-                  u_v_r_cons1[where r' = "{}" and w' = "{}", simplified]
-                  u_v_r_empty; simp?)
-   apply (rule upd_val_rel_bang(1); simp)
-  apply clarsimp
-  apply (frule_tac r = "(ra \<union> wa) \<union> ro"  and w = "{}" in mono_correspondence(1)[rotated 3]; simp?)
-   apply (intro u_v_matches_some[where r' = "{}" and w' = "{}", simplified]
-                  u_v_matches_empty[where \<tau>s = "[]", simplified]
-                  u_v_struct
-                  u_v_r_cons1[where w' = "{}", simplified]
-                  u_v_r_cons1[where r' = "{}" and w' = "{}", simplified]
-                  u_v_r_empty; simp?)
-   apply (rule upd_val_rel_bang(1); simp)
-  apply clarsimp
-  apply (erule u_v_primE'; clarsimp)
-  apply (frule_tac r = "(ra \<union> wa) \<union> ro"  and w = "{}" and v' = "VPrim (LBool True)" in mono_correspondence(1)[rotated 3]; simp?)
-  apply (intro u_v_matches_some[where r' = "{}" and w' = "{}", simplified]
-                  u_v_matches_empty[where \<tau>s = "[]", simplified]
-                  u_v_struct
-                  u_v_r_cons1[where w' = "{}", simplified]
-                  u_v_r_cons1[where r' = "{}" and w' = "{}", simplified]
-                  u_v_r_empty; simp?)
-   apply (rule upd_val_rel_bang(1); simp)
-  apply clarsimp
-  apply (erule u_v_primE; clarsimp)
-  done
-*)
 end
