cogent/examples/repeat/RepeatUpdate.thy
@@ -1,15 +1,28 @@
 theory RepeatUpdate
-  imports RepeatAssm
+  imports UpdateSemHelper
 begin
 
-section "definitions" 
+section "Repeat loop definitions" 
 
-overloading \<xi>0 \<equiv> \<xi>_0
-begin
-definition \<xi>0 :: "(funtyp, abstyp, ptrtyp) uabsfuns"
-  where
-"\<xi>0 f x y = False"
-end
+text "Main body:
+  Summary:
+    Does at most @{term \<open>n::nat\<close>} iterations and apply @{term \<open>g ::'f expr\<close>} to update the input
+    accumulator and heap. If @{term \<open>f ::'f expr\<close>} returns @{term True} then terminate early.
+  Arguments:
+    @{term \<open>\<xi>'::('f, 'a, 'l) uabsfuns\<close>} is a partial mapping from abstract function names to their specifications,
+    @{term \<open>n::nat\<close>} is a natural number that is recursed on, i.e. terminate if 0 else subtract 1, apply body and repeat ,
+    @{term \<open>f ::'f expr\<close>} is a Cogent expression that is used to check if the loop should terminate early,
+    @{term \<open>g ::'f expr\<close>} is a Cogent expression that is used to update the heap and the accumulator,
+    @{term \<open>\<sigma>::('f, 'a, 'l) store\<close>} is the input heap that is updated each loop iteration,
+    @{term \<open>\<sigma>'::('f, 'a, 'l) store\<close>} is the output heap,
+    @{term \<open>\<tau>a::type\<close>} is the Cogent type of the accumulator,
+    @{term \<open>acc::('f, 'a, 'l) uval\<close>} is the accumulator that is updated each loop iteration,
+    @{term \<open>\<tau>o::type\<close>} is the Cogent type of the observer,
+    @{term \<open>obsv::('f, 'a, 'l) uval\<close>} is the observer that does not change throughout the loop,
+    @{term \<open>ret::('f, 'a, 'l) uval\<close>} is the is the output accumulator value.
+  Output:
+    @{term True} if the loop evaluates to the output heap and accumulator,
+    @{term False} otherwise."
 
 fun urepeat_bod
   where
@@ -22,18 +35,13 @@ fun urepeat_bod
         \<turnstile> (\<sigma>, App g (Var 0)) \<Down>! (\<sigma>'', acc')) \<and>
       urepeat_bod \<xi>' n f g \<sigma>'' \<sigma>' \<tau>a acc' \<tau>o obsv ret)))"
 
-
-fun is_uvalfun
-  where
-"is_uvalfun (UFunction _ _) = True" |
-"is_uvalfun (UAFunction _ _) = True" |
-"is_uvalfun _ = False"
-
-fun uvalfun_to_expr
-  where
-"uvalfun_to_expr (UFunction f ts) = Fun f ts" |
-"uvalfun_to_expr (UAFunction f ts) = AFun f ts" |
-"uvalfun_to_expr _ = undefined"
+text "Wrapper with extra checks:
+  Summary:
+    Checks the arguments are of the correct form and type and then passes these to
+    @{term urepeat_bod} with minor processing.
+  Checks:
+    * The observer type has been banged, i.e. is read-only or is drop-able.
+    * The functions f and g are of the correct type and form."
 
 definition urepeat
   where
@@ -51,16 +59,11 @@ definition urepeat
       \<turnstile> (App (uvalfun_to_expr g) (Var 0)) : \<tau>a) \<and>
     urepeat_bod \<xi>' (unat n) (uvalfun_to_expr f) (uvalfun_to_expr g) \<sigma> \<sigma>' \<tau>a acc \<tau>o obsv ret)"
 
-overloading \<xi>1 \<equiv> \<xi>_1
-begin
-definition \<xi>1 :: "(funtyp, abstyp, ptrtyp) uabsfuns"
-  where
-"\<xi>1 f x y = (if f = ''repeat_0'' then urepeat \<Xi> \<xi>_0 abbreviatedType1 (TPrim (Num U64)) x y  else \<xi>_0 f x y)"
-end
-
-section "theorems"
+section "Repeat loop lemmas"
 
 context update_sem begin
+
+subsection "Preservation and frame constraint satisfaction"
 
 lemma urepeat_bod_preservation:
   "\<lbrakk>proc_ctx_wellformed \<Xi>';
@@ -77,6 +80,7 @@ lemma urepeat_bod_preservation:
    apply (intro exI conjI, assumption, blast, rule frame_id)
   apply (rename_tac \<xi>' n f g \<sigma> \<sigma>' \<tau>a acc \<tau>o obsv ret ra wa)
   apply clarsimp
+  apply (rename_tac b)
   apply (case_tac b; clarsimp)
    apply (intro exI conjI, assumption, blast, rule frame_id)
   apply (drule_tac x = False in meta_spec; clarsimp)
@@ -103,45 +107,6 @@ lemma urepeat_bod_preservation:
    apply blast
   apply (rule frame_trans; simp?)
   done
-
-lemma urepeat_bod_early_termination:
-  "\<lbrakk>urepeat_bod \<xi>' i f g \<sigma> \<sigma>' \<tau>a acc \<tau>o obsv ret; i < n;
-    \<xi>', [URecord [(ret, type_repr (bang \<tau>a)), (obsv, type_repr \<tau>o)]]  \<turnstile> (\<sigma>', App f (Var 0)) \<Down>! (\<sigma>', UPrim (LBool True))\<rbrakk>
-    \<Longrightarrow> urepeat_bod \<xi>' n f g \<sigma> \<sigma>' \<tau>a acc \<tau>o obsv ret"
-  apply (induct arbitrary: i rule: urepeat_bod.induct[of _ \<xi>' n f g \<sigma> \<sigma>' \<tau>a acc \<tau>o obsv ret])
-   apply clarsimp
-  apply clarsimp
-  apply (rename_tac i)
-  apply (case_tac i; clarsimp)
-   apply blast
-  apply (case_tac b; clarsimp)
-   apply blast
-  apply (rename_tac ret nat b \<sigma>'' acc')
-  apply (rule_tac x = b in exI)
-  apply (rule conjI; clarsimp)
-  apply (intro exI conjI; assumption)
-  done
-
-declare urepeat_bod.simps[simp del]
-lemma urepeat_bod_step:
-  "\<lbrakk>\<xi>', [URecord [(ret, type_repr (bang \<tau>a)), (obsv, type_repr \<tau>o)]] \<turnstile> (\<sigma>', App f (Var 0)) \<Down>! (\<sigma>', UPrim (LBool False));
-    \<not>(\<xi>', [URecord [(ret, type_repr (bang \<tau>a)), (obsv, type_repr \<tau>o)]] \<turnstile> (\<sigma>', App f (Var 0)) \<Down>! (\<sigma>', UPrim (LBool True)));
-    \<xi>', [URecord [(ret, type_repr \<tau>a), (obsv, type_repr \<tau>o)]] \<turnstile> (\<sigma>', App g (Var 0)) \<Down>! (\<sigma>'', ret');
-    urepeat_bod \<xi>' n f g \<sigma> \<sigma>' \<tau>a acc \<tau>o obsv ret\<rbrakk> 
-    \<Longrightarrow> urepeat_bod \<xi>' (Suc n) f g \<sigma> \<sigma>'' \<tau>a acc \<tau>o obsv ret'"
-  apply (induct arbitrary: \<sigma>'' ret' rule: urepeat_bod.induct[of _ \<xi>' n f g \<sigma> \<sigma>' \<tau>a acc \<tau>o obsv ret])
-   apply (clarsimp simp: urepeat_bod.simps)
-  apply clarsimp
-  apply (erule urepeat_bod.elims; clarsimp)
-  apply (rename_tac \<sigma>'' ret' \<xi> n f g \<sigma> \<sigma>' \<tau>a acc \<tau>o obsv ret b)
-  apply (case_tac b; clarsimp)
-  apply (drule_tac x = b in meta_spec; clarsimp)
-  apply (elim meta_allE meta_impE, assumption, assumption)
-  apply (subst urepeat_bod.simps; clarsimp)
-  apply (rule_tac x = b in exI; clarsimp)
-  apply (intro exI conjI; assumption)
-  done
-declare urepeat_bod.simps[simp]
 
 lemma urepeat_preservation:
   "\<And>\<sigma> \<sigma>' v v' r w.
@@ -175,131 +140,49 @@ lemma urepeat_preservation:
   apply blast
   done
 
-end (* of context *)
+subsection "Early termination and step lemmas"
 
-context update_sem_init begin
-
-lemma \<xi>_0_matchesu_\<Xi>:
-  "\<xi>_0 matches-u \<Xi>'"
-  unfolding proc_env_matches_ptrs_def \<xi>0_def
-  by clarsimp
- 
-lemma \<xi>_1_matchesu_\<Xi>:
-  "\<xi>_1 matches-u \<Xi>"
-  unfolding proc_env_matches_ptrs_def \<xi>1_def
-  apply clarsimp
-  apply (rule conjI)
-   apply clarsimp
-   apply (subst (asm) \<Xi>_def; clarsimp)
-   apply (clarsimp simp: repeat_0_type_def)
-   apply (rule urepeat_preservation[OF proc_ctx_wellformed_\<Xi> \<xi>_0_matchesu_\<Xi>]; (simp add: abbreviated_type_defs)?)
-  apply (clarsimp simp: \<xi>0_def)
-  done
-end (* of context *)
-
-
-
-(*
-fun repeat_bod
-  where
-"repeat_bod _ 0 _ _ \<sigma> \<sigma>' _ acc _ _ ret = (\<sigma> = \<sigma>' \<and> acc = ret)" |
-"repeat_bod \<xi>' (Suc n) f g \<sigma> \<sigma>' \<tau>a acc \<tau>o obsv ret =
-  (if (\<xi>' , [URecord [(acc, type_repr (bang \<tau>a)), (obsv, type_repr \<tau>o)]] 
-      \<turnstile> (\<sigma>, App f (Var 0)) \<Down>! (\<sigma>, UPrim (LBool True))) \<and>
-      \<not>(\<xi>' , [URecord [(acc, type_repr (bang \<tau>a)), (obsv, type_repr \<tau>o)]] 
-      \<turnstile> (\<sigma>, App f (Var 0)) \<Down>! (\<sigma>, UPrim (LBool False)))
-    then \<sigma> = \<sigma>' \<and> acc = ret
-  else if (\<xi>' , [URecord [(acc, type_repr (bang \<tau>a)), (obsv, type_repr \<tau>o)]] 
-      \<turnstile> (\<sigma>, App f (Var 0)) \<Down>! (\<sigma>, UPrim (LBool False))) \<and>
-      \<not>(\<xi>' , [URecord [(acc, type_repr (bang \<tau>a)), (obsv, type_repr \<tau>o)]] 
-      \<turnstile> (\<sigma>, App f (Var 0)) \<Down>! (\<sigma>, UPrim (LBool True)))
-    then (\<exists>\<sigma>'' acc'. (\<xi>' , [URecord [(acc, type_repr \<tau>a), (obsv, type_repr \<tau>o)]] 
-        \<turnstile> (\<sigma>, App g (Var 0)) \<Down>! (\<sigma>'', acc')) \<and>
-      repeat_bod \<xi>' n f g \<sigma>'' \<sigma>' \<tau>a acc' \<tau>o obsv ret)
-  else False)"
-
-context Generated begin
-
-lemma repeat_bod_preservation:
-  "\<lbrakk>proc_ctx_wellformed \<Xi>';
-    \<xi>' matches-u \<Xi>';
-    \<Xi>', \<sigma> \<turnstile> acc :u \<tau>a \<langle>ra, wa\<rangle>;
-    \<Xi>', \<sigma> \<turnstile> obsv :u \<tau>o \<langle>ro, {}\<rangle>;
-    ro \<inter> wa = {};
-    repeat_bod \<xi>' n f g \<sigma> \<sigma>' \<tau>a acc \<tau>o obsv ret;
-    \<Xi>', [], [option.Some (TRecord [(''acc'', \<tau>a, Present), (''obsv'', \<tau>o, Present)] Unboxed)] \<turnstile> (App g (Var 0)) : \<tau>a\<rbrakk>
-      \<Longrightarrow> \<exists>r' w'. \<Xi>', \<sigma>' \<turnstile> ret :u \<tau>a \<langle>r', w'\<rangle> \<and> r' \<subseteq> (ra \<union> ro) \<and> frame \<sigma> wa \<sigma>' w'"
-  apply (induct arbitrary: ra wa rule: repeat_bod.induct[of _ \<xi>' n f g \<sigma> \<sigma>' \<tau>a acc \<tau>o obsv ret])
-   apply (rename_tac \<xi>' f g \<sigma> \<sigma>' \<tau>a acc \<tau>o obsv ret ra wa)
-   apply clarsimp
-   apply (intro exI conjI, assumption, blast, rule frame_id)
-  apply (rename_tac \<xi>' n f g \<sigma> \<sigma>' \<tau>a acc \<tau>o obsv ret ra wa)
-  apply (clarsimp split: if_splits)
-   apply (intro exI conjI, assumption, blast, rule frame_id)
-  apply (rename_tac \<sigma>'' acc')
-  apply (drule_tac x = \<sigma>'' and y = acc' in meta_spec2)
-  apply clarsimp
-  apply (drule_tac \<gamma> = "[URecord [(acc, type_repr \<tau>a), (obsv, type_repr \<tau>o)]]" and
-      \<sigma>' = \<sigma>'' and v = acc' and r = "ra \<union> ro" and w = wa in preservation_mono(1)[rotated -1]; simp?)
-   apply (intro matches_ptrs_some[where r' = "{}" and w' = "{}", simplified]
-      matches_ptrs_empty[where \<tau>s = "[]", simplified])
-   apply (rule u_t_struct; simp?) 
-   apply (intro u_t_r_cons1[where  r' = ro and w' = "{}", simplified]
-      u_t_r_cons1[where  r' = "{}" and w' = "{}", simplified] u_t_r_empty; simp?)
-   apply blast
-  apply clarsimp
-  apply (rename_tac r' w')
-  apply (drule_tac x = r' and y = w' in meta_spec2; simp)
-  apply (erule meta_impE)
-   apply (drule_tac u = obsv in uval_typing_frame(1); simp?)
-  apply (drule meta_mp)
-   apply (drule_tac v = obsv in frame_noalias_uval_typing'(2); simp?)
-  apply clarsimp
-  apply (rename_tac r'' w'')
-  apply (intro exI conjI, assumption)
-   apply blast
-  apply (rule frame_trans; simp?)
-  done
-
-
-lemma repeat_bod_early_termination:
-  "\<lbrakk>repeat_bod \<xi>' i f g \<sigma> \<sigma>' \<tau>a acc \<tau>o obsv ret; i < n;
-    \<xi>', [URecord [(ret, type_repr (bang \<tau>a)), (obsv, type_repr \<tau>o)]]  \<turnstile> (\<sigma>', App f (Var 0)) \<Down>! (\<sigma>', UPrim (LBool True));
-    \<not>(\<xi>', [URecord [(ret, type_repr (bang \<tau>a)), (obsv, type_repr \<tau>o)]]  \<turnstile> (\<sigma>', App f (Var 0)) \<Down>! (\<sigma>', UPrim (LBool False)))\<rbrakk>
-    \<Longrightarrow> repeat_bod \<xi>' n f g \<sigma> \<sigma>' \<tau>a acc \<tau>o obsv ret"
-  apply (induct arbitrary: i rule: repeat_bod.induct[of _ \<xi>' n f g \<sigma> \<sigma>' \<tau>a acc \<tau>o obsv ret])
+lemma urepeat_bod_early_termination:
+  "\<lbrakk>urepeat_bod \<xi>' i f g \<sigma> \<sigma>' \<tau>a acc \<tau>o obsv ret; i < n;
+    \<xi>', [URecord [(ret, type_repr (bang \<tau>a)), (obsv, type_repr \<tau>o)]]  \<turnstile> (\<sigma>', App f (Var 0)) \<Down>! (\<sigma>', UPrim (LBool True))\<rbrakk>
+    \<Longrightarrow> urepeat_bod \<xi>' n f g \<sigma> \<sigma>' \<tau>a acc \<tau>o obsv ret"
+  apply (induct arbitrary: i rule: urepeat_bod.induct[of _ \<xi>' n f g \<sigma> \<sigma>' \<tau>a acc \<tau>o obsv ret])
    apply clarsimp
   apply clarsimp
   apply (rename_tac i)
+  apply (case_tac i; clarsimp)
+   apply blast
+  apply (rename_tac b)
+  apply (case_tac b; clarsimp)
+   apply blast
+  apply (rename_tac ret nat b \<sigma>'' acc')
+  apply (rule_tac x = b in exI)
   apply (rule conjI; clarsimp)
-   apply (case_tac i; clarsimp)
-   apply (intro exI conjI; assumption)
-  apply (rule conjI)
-   apply clarsimp
-   apply (case_tac i; clarsimp)
-  apply (rule conjI; clarsimp)
-   apply (case_tac i; clarsimp split: if_splits)
-  apply (case_tac i; clarsimp split: if_splits)
+  apply (intro exI conjI; assumption)
   done
 
-lemma repeat_bod_step:
+declare urepeat_bod.simps[simp del]
+lemma urepeat_bod_step:
   "\<lbrakk>\<xi>', [URecord [(ret, type_repr (bang \<tau>a)), (obsv, type_repr \<tau>o)]] \<turnstile> (\<sigma>', App f (Var 0)) \<Down>! (\<sigma>', UPrim (LBool False));
     \<not>(\<xi>', [URecord [(ret, type_repr (bang \<tau>a)), (obsv, type_repr \<tau>o)]] \<turnstile> (\<sigma>', App f (Var 0)) \<Down>! (\<sigma>', UPrim (LBool True)));
     \<xi>', [URecord [(ret, type_repr \<tau>a), (obsv, type_repr \<tau>o)]] \<turnstile> (\<sigma>', App g (Var 0)) \<Down>! (\<sigma>'', ret');
-    repeat_bod \<xi>' n f g \<sigma> \<sigma>' \<tau>a acc \<tau>o obsv ret\<rbrakk> 
-    \<Longrightarrow> repeat_bod \<xi>' (Suc n) f g \<sigma> \<sigma>'' \<tau>a acc \<tau>o obsv ret'"
-  apply (induct arbitrary: \<sigma>'' ret' rule: repeat_bod.induct[of _ \<xi>' n f g \<sigma> \<sigma>' \<tau>a acc \<tau>o obsv ret])
-   apply clarsimp
-  apply (simp del: repeat_bod.simps)
-  apply (erule repeat_bod.elims; clarsimp simp del: repeat_bod.simps split: if_splits)
-  apply (subst repeat_bod.simps; clarsimp simp del: repeat_bod.simps)
-  apply (rename_tac \<sigma>'' ret' \<xi>' n f g \<sigma> \<sigma>m \<tau>a acc \<tau>o obsv ret \<sigma>' acc')
-  apply (drule_tac x = \<sigma>' and y = acc' in meta_spec2)
-  apply (drule_tac x = \<sigma>'' and y = ret' in meta_spec2)
-  apply (clarsimp simp del: repeat_bod.simps)
+    urepeat_bod \<xi>' n f g \<sigma> \<sigma>' \<tau>a acc \<tau>o obsv ret\<rbrakk> 
+    \<Longrightarrow> urepeat_bod \<xi>' (Suc n) f g \<sigma> \<sigma>'' \<tau>a acc \<tau>o obsv ret'"
+  apply (induct arbitrary: \<sigma>'' ret' rule: urepeat_bod.induct[of _ \<xi>' n f g \<sigma> \<sigma>' \<tau>a acc \<tau>o obsv ret])
+   apply (clarsimp simp: urepeat_bod.simps)
+   apply blast
+  apply clarsimp
+  apply (erule urepeat_bod.elims; clarsimp)
+  apply (rename_tac \<sigma>'' ret' \<xi> n f g \<sigma> \<sigma>' \<tau>a acc \<tau>o obsv ret b)
+  apply (case_tac b; clarsimp)
+  apply (drule_tac x = b in meta_spec; clarsimp)
+  apply (elim meta_allE meta_impE, assumption, assumption)
+  apply (subst urepeat_bod.simps; clarsimp)
+  apply (rule_tac x = b in exI; clarsimp)
   apply (intro exI conjI; assumption)
   done
+declare urepeat_bod.simps[simp]
+
 end (* of context *)
-*)
 
 end
