cogent/examples/repeat/RepeatValue.thy
@@ -1,6 +1,24 @@
 theory RepeatValue
-  imports RepeatAssm
+  imports ValueSemHelper
 begin
+
+section "Repeat loop definitions"
+
+text "Main body:
+  Summary:
+    Does at most @{term \<open>n::nat\<close>} iterations and apply @{term \<open>g ::'f expr\<close>} to update the input
+    accumulator. If @{term \<open>f ::'f expr\<close>} returns @{term True} then terminate early.
+  Arguments:
+    @{term \<open>\<xi>'::('f, 'a) vabsfuns\<close>} is a partial mapping from abstract function names to their specifications,
+    @{term \<open>n::nat\<close>} is a natural number that is recursed on, i.e. terminate if 0 else subtract 1, apply body and repeat ,
+    @{term \<open>f ::'f expr\<close>} is a Cogent expression that is used to check if the loop should terminate early,
+    @{term \<open>g ::'f expr\<close>} is a Cogent expression that is used to update the accumulator,
+    @{term \<open>acc::('f, 'a) vval\<close>} is the accumulator that is updated each loop iteration,
+    @{term \<open>obsv::('f, 'a) vval\<close>} is the observer that does not change throughout the loop,
+    @{term \<open>ret::('f, 'a) vval\<close>} is the is the output accumulator value.
+  Output:
+    @{term True} if the loop evaluates to the output accumulator,
+    @{term False} otherwise."
 
 fun vrepeat_bod
   where
@@ -11,19 +29,14 @@ fun vrepeat_bod
      else (\<exists>acc'. (\<xi>' , [VRecord [acc, obsv]] \<turnstile> App g (Var 0) \<Down> acc') \<and>
       vrepeat_bod \<xi>' n f g acc' obsv ret)))"
 
-fun is_vvalfun
-  where
-"is_vvalfun (VFunction _ _) = True" |
-"is_vvalfun (VAFunction _ _) = True" |
-"is_vvalfun _  = False"
-
-fun vvalfun_to_expr
-  where
-"vvalfun_to_expr (VFunction f ts) = Fun f ts" |
-"vvalfun_to_expr (VAFunction f ts) = AFun f ts" |
-"vvalfun_to_expr _ = undefined"
-
 context value_sem begin
+
+text "Wrapper with extra checks:
+  Summary:
+    Checks the arguments are of the correct form and type and then passes these to
+    @{term vrepeat_bod} with minor processing.
+  Checks:
+    * The functions f and g are of the correct type and form."
 
 definition vrepeat
   where
@@ -41,13 +54,7 @@ definition vrepeat
       \<turnstile> (App (vvalfun_to_expr g) (Var 0)) : \<tau>a) \<and>
     vrepeat_bod \<xi>' (unat n) (vvalfun_to_expr f) (vvalfun_to_expr g) acc obsv ret)"
 
-definition \<xi>m0 :: "'b \<Rightarrow> ('b, 'a) vval \<Rightarrow> ('b, 'a) vval \<Rightarrow> bool "
-  where
-"\<xi>m0 f x y = False"
-
-definition \<xi>m1 :: "funtyp \<Rightarrow> (funtyp, 'a) vval \<Rightarrow> (funtyp, 'a) vval \<Rightarrow> bool "
-  where
-"\<xi>m1 f x y = (if f = ''repeat_0'' then vrepeat \<Xi> \<xi>m0 abbreviatedType1 (TPrim (Num U64)) x y else \<xi>m0 f x y)"
+section "Preservation lemmas"
 
 lemma vrepeat_bod_preservation:
   "\<lbrakk>proc_ctx_wellformed \<Xi>';
@@ -61,6 +68,7 @@ lemma vrepeat_bod_preservation:
    apply clarsimp
   apply (clarsimp split: if_splits)
   apply (erule disjE; clarsimp)
+  apply (rename_tac \<xi>' n f g acc obsv ret b acc')
   apply (case_tac b; clarsimp)
   apply (drule_tac x = b in meta_spec; clarsimp)
   apply (drule_tac x = acc' in meta_spec; clarsimp)
@@ -71,46 +79,6 @@ lemma vrepeat_bod_preservation:
    apply (rule v_t_r_empty)
   apply (drule meta_mp; simp)
   done
-
-lemma vrepeat_bod_early_termination:
-  "\<lbrakk>vrepeat_bod \<xi>' i f g acc obsv ret; i < n;
-    \<xi>' , [VRecord [ret, obsv]] \<turnstile> App f (Var 0) \<Down> VPrim (LBool True)\<rbrakk>
-    \<Longrightarrow> vrepeat_bod \<xi>' n f g acc obsv ret"
-  apply (induct arbitrary: i rule: vrepeat_bod.induct[of _ \<xi>' n f g acc obsv ret])
-   apply clarsimp
-  apply clarsimp
-  apply (rename_tac i)
-  apply (case_tac i; clarsimp)
-   apply blast
-  apply (case_tac b; clarsimp)
-   apply blast
-  apply (rename_tac ret nat b acc')
-  apply (rule_tac x = b in exI)
-  apply (rule conjI; clarsimp)
-  apply (intro exI conjI; assumption)
-  done
-
-declare vrepeat_bod.simps[simp del]
-lemma vrepeat_bod_step:
-  "\<lbrakk>\<xi>', [VRecord [ret, obsv]] \<turnstile> App f (Var 0) \<Down> VPrim (LBool False);
-    \<not>(\<xi>', [VRecord [ret, obsv]] \<turnstile> App f (Var 0) \<Down> VPrim (LBool True));
-    \<xi>', [VRecord [ret, obsv]] \<turnstile> App g (Var 0) \<Down> ret';
-    vrepeat_bod \<xi>' n f g acc obsv ret\<rbrakk> 
-    \<Longrightarrow> vrepeat_bod \<xi>' (Suc n) f g acc obsv ret'"
-  apply (induct arbitrary: ret' rule: vrepeat_bod.induct[of _ \<xi>' n f g acc obsv ret])
-  apply (simp only: vrepeat_bod.simps)
-   apply (clarsimp simp: vrepeat_bod.simps)
-  apply clarsimp
-  apply (erule vrepeat_bod.elims; clarsimp)
-  apply (rename_tac ret' \<xi> n f g acc obsv ret b)
-  apply (case_tac b; clarsimp)
-  apply (drule_tac x = b in meta_spec; clarsimp)
-  apply (elim meta_allE meta_impE, assumption, assumption)
-  apply (subst vrepeat_bod.simps; clarsimp)
-  apply (rule_tac x = b in exI; clarsimp)
-  apply (intro exI conjI; assumption)
-  done
-declare vrepeat_bod.simps[simp]
 
 lemma vrepeat_preservation:
   "\<And>v v'.
@@ -131,57 +99,50 @@ lemma vrepeat_preservation:
   apply (rule vrepeat_bod_preservation; simp)
   done
 
-lemma \<xi>m0_matches_\<Xi>:
-  "\<xi>m0 matches \<Xi>'"
-  unfolding proc_env_matches_def \<xi>m0_def
-  by clarsimp
+section "Early termination and step lemmas"
 
-lemma \<xi>m1_matches_\<Xi>:
-  "\<xi>m1 matches \<Xi>"
-  unfolding proc_env_matches_def \<xi>m1_def
-  apply clarsimp
-  apply (rule conjI; clarsimp)
-   apply (subst (asm) \<Xi>_def; clarsimp simp: repeat_0_type_def)
-   apply (rule vrepeat_preservation[OF proc_ctx_wellformed_\<Xi> \<xi>m0_matches_\<Xi>]; (simp add: abbreviated_type_defs)?)
-  apply (clarsimp simp: \<xi>m0_def)
-  done
-
-end (* of context *)
-
-(*
-fun repeat_bod'
-  where
-"repeat_bod' _ 0 _ _ acc _ ret = (acc = ret)" |
-"repeat_bod' \<xi>' (Suc n) f g acc obsv ret =
-  (if (\<xi>' , [VRecord [acc, obsv]] \<turnstile> App f (Var 0) \<Down> VPrim (LBool True)) \<and>
-      \<not>(\<xi>' , [VRecord [acc, obsv]] \<turnstile> App f (Var 0) \<Down> VPrim (LBool False))
-    then acc = ret
-  else if (\<xi>' , [VRecord [acc, obsv]] \<turnstile> App f (Var 0) \<Down> VPrim (LBool False)) \<and>
-      \<not>(\<xi>' , [VRecord [acc, obsv]] \<turnstile> App f (Var 0) \<Down> VPrim (LBool True))
-    then (\<exists>acc'. (\<xi>' , [VRecord [acc, obsv]] \<turnstile> App g (Var 0) \<Down> acc') \<and>
-      repeat_bod' \<xi>' n f g acc' obsv ret)
-  else False)"
-
-context shallow begin
-lemma repeat_bod'_preservation:
-  "\<lbrakk>proc_ctx_wellformed \<Xi>';
-    \<xi>' matches \<Xi>';
-    \<Xi>' \<turnstile> acc :v \<tau>a;
-    \<Xi>' \<turnstile> obsv :v \<tau>o;
-    repeat_bod' \<xi>' n f g acc obsv ret;
-    \<Xi>', [], [option.Some (TRecord [(''acc'', \<tau>a, Present), (''obsv'', \<tau>o, Present)] Unboxed)] \<turnstile> (App g (Var 0)) : \<tau>a\<rbrakk>
-      \<Longrightarrow> \<Xi>' \<turnstile> ret :v \<tau>a"
-  apply (induct arbitrary: rule: repeat_bod'.induct[of _ \<xi>' n f g acc obsv ret])
+lemma vrepeat_bod_early_termination:
+  "\<lbrakk>vrepeat_bod \<xi>' i f g acc obsv ret; i < n;
+    \<xi>' , [VRecord [ret, obsv]] \<turnstile> App f (Var 0) \<Down> VPrim (LBool True)\<rbrakk>
+    \<Longrightarrow> vrepeat_bod \<xi>' n f g acc obsv ret"
+  apply (induct arbitrary: i rule: vrepeat_bod.induct[of _ \<xi>' n f g acc obsv ret])
    apply clarsimp
-  apply (clarsimp split: if_splits)
-  apply (drule_tac x = acc' in meta_spec; clarsimp)
-  apply (drule_tac \<gamma> = "[VRecord [acc, obsv]]" and v = acc' in preservation(1)[of "[]" "[]", simplified]; simp?)
-   apply (clarsimp simp: matches_def)
-   apply (rule v_t_record; simp?)
-   apply (rule v_t_r_cons1; simp?)+
-   apply (rule v_t_r_empty)
-  apply (drule meta_mp; simp)
+  apply clarsimp
+  apply (rename_tac i)
+  apply (case_tac i; clarsimp)
+   apply blast
+  apply (rename_tac b)
+  apply (case_tac b; clarsimp)
+   apply blast
+  apply (rename_tac ret nat b acc')
+  apply (rule_tac x = b in exI)
+  apply (rule conjI; clarsimp)
+  apply (intro exI conjI; assumption)
   done
+
+declare vrepeat_bod.simps[simp del]
+lemma vrepeat_bod_step:
+  "\<lbrakk>\<xi>', [VRecord [ret, obsv]] \<turnstile> App f (Var 0) \<Down> VPrim (LBool False);
+    \<not>(\<xi>', [VRecord [ret, obsv]] \<turnstile> App f (Var 0) \<Down> VPrim (LBool True));
+    \<xi>', [VRecord [ret, obsv]] \<turnstile> App g (Var 0) \<Down> ret';
+    vrepeat_bod \<xi>' n f g acc obsv ret\<rbrakk> 
+    \<Longrightarrow> vrepeat_bod \<xi>' (Suc n) f g acc obsv ret'"
+  apply (induct arbitrary: ret' rule: vrepeat_bod.induct[of _ \<xi>' n f g acc obsv ret])
+  apply (simp only: vrepeat_bod.simps)
+   apply (clarsimp simp: vrepeat_bod.simps)
+   apply blast
+  apply clarsimp
+  apply (erule vrepeat_bod.elims; clarsimp)
+  apply (rename_tac ret' \<xi> n f g acc obsv ret b)
+  apply (case_tac b; clarsimp)
+  apply (drule_tac x = b in meta_spec; clarsimp)
+  apply (elim meta_allE meta_impE, assumption, assumption)
+  apply (subst vrepeat_bod.simps; clarsimp)
+  apply (rule_tac x = b in exI; clarsimp)
+  apply (intro exI conjI; assumption)
+  done
+declare vrepeat_bod.simps[simp]
+
 end (* of context *)
-*)
+
 end
